coq/proof/SoundForgetMemory.v
@@ -28,6 +28,12 @@ Require Import SoundForget.
 
 Set Implicit Arguments.
 
+(* TODO: move *)
+Lemma some_injective A (a b:A):
+  Some a = Some b -> a = b.
+Proof.
+  congruence.
+Qed.
 
 Inductive mem_change : Type :=
 | mem_change_alloc
@@ -213,12 +219,9 @@ Lemma mem_change_inject_no_private_parent_tgt
       (INJECT: mem_change_inject conf_src conf_tgt invmem mc_src mc_tgt)
   : mem_change_no_private_parent conf_tgt mc_tgt invmem.(InvMem.Rel.tgt).(InvMem.Unary.private_parent).
 Proof.
-  inv SEM.
-  inv TGT.
-  inv INJECT; try econs; ii; ss; inv UPDATE.
-  - exploit PRIVATE_PARENT; eauto. i. des.
-    hexploit gv_inject_ptr_public_tgt; try apply PTR; eauto.
-  - exploit PRIVATE_PARENT; eauto. i. des.
+  inv SEM. inv TGT.
+  inv INJECT; try econs; ii; ss; inv UPDATE;
+    exploit PRIVATE_PARENT; eauto; i; des;
     hexploit gv_inject_ptr_public_tgt; try apply PTR; eauto.
 Qed.
 
@@ -300,42 +303,24 @@ Lemma unary_sem_eq_locals_mem
       conf st0 st1 invst0 invmem0 inv0
       (LOCALS_EQ: Locals (EC st0) = Locals (EC st1))
       (MEM_EQ : Mem st0 = Mem st1)
-  : <<SEM_ST0: InvState.Unary.sem conf st0 invst0 invmem0 inv0>> <->
-    <<SEM_ST1: InvState.Unary.sem conf st1 invst0 invmem0 inv0>>.
+      (STATE: InvState.Unary.sem conf st0 invst0 invmem0 inv0)
+  : InvState.Unary.sem conf st1 invst0 invmem0 inv0.
 Proof.
-  split; intro STATE.
-  { inv STATE.
-    econs.
-    - ii.
-      exploit LESSDEF; eauto.
-      { erewrite sem_expr_eq_locals_mem; eauto. }
-      i. des.
-      esplits; eauto.
-      erewrite sem_expr_eq_locals_mem; eauto.
-    - inv NOALIAS.
-      econs; i; [exploit DIFFBLOCK | exploit NOALIAS0]; eauto;
-        erewrite sem_valueT_eq_locals; eauto.
-    - ii. exploit UNIQUE; eauto. intro UNIQ_X. inv UNIQ_X.
-      econs; try rewrite <- LOCALS_EQ; try rewrite <- MEM_EQ; eauto.
-    - ii. exploit PRIVATE; eauto.
-      erewrite sem_idT_eq_locals; eauto.
-  }
-  { inv STATE.
-    econs.
-    - ii.
-      exploit LESSDEF; eauto.
-      { erewrite sem_expr_eq_locals_mem; eauto. }
-      i. des.
-      esplits; eauto.
-      erewrite sem_expr_eq_locals_mem; eauto.
-    - inv NOALIAS.
-      econs; i; [exploit DIFFBLOCK | exploit NOALIAS0]; eauto;
-        erewrite sem_valueT_eq_locals; eauto.
-    - ii. exploit UNIQUE; eauto. intro UNIQ_X. inv UNIQ_X.
-      econs; try rewrite  LOCALS_EQ; try rewrite MEM_EQ; eauto.
-    - ii. exploit PRIVATE; eauto.
-      erewrite sem_idT_eq_locals; eauto.
-  }
+  inv STATE.
+  econs.
+  - ii.
+    exploit LESSDEF; eauto.
+    { erewrite sem_expr_eq_locals_mem; eauto. }
+    i. des.
+    esplits; eauto.
+    erewrite sem_expr_eq_locals_mem; eauto.
+  - inv NOALIAS.
+    econs; i; [exploit DIFFBLOCK | exploit NOALIAS0]; eauto;
+      erewrite sem_valueT_eq_locals; eauto.
+  - ii. exploit UNIQUE; eauto. intro UNIQ_X. inv UNIQ_X.
+    econs; try rewrite <- LOCALS_EQ; try rewrite <- MEM_EQ; eauto.
+  - ii. exploit PRIVATE; eauto.
+    erewrite sem_idT_eq_locals; eauto.
 Qed.
 
 (* soundness proof *)
@@ -372,27 +357,67 @@ Lemma step_mem_change
     <<STATE_EQUIV: states_mem_change conf st0.(Mem) st1.(Mem) mc>>.
 Proof.
   inv STEP; ss;
-    try by inv CMD;
-    esplits; ss; econs; eauto.
-  - admit. (* not malloc *)
-  - inv CMD.
-    esplits; ss.
-    + des_ifs.
-    + esplits; eauto.
-    + econs; eauto.
-  - inv CMD.
-    esplits; ss.
-    + des_ifs.
-    + esplits; eauto.
-    + econs; eauto.
-  - inv CMD.
-    esplits; ss.
-    + des_ifs.
-    + esplits; eauto.
-    + econs; eauto.
+    try (by inv CMD;
+         esplits; ss; econs; eauto);
+    try (by inv CMD;
+         esplits; ss; [des_ifs | esplits | econs]; eauto).
+  admit. (* not malloc *)
 Admitted.
 
-Lemma malloc_nextblock
+Ltac exploit_inject_value :=
+  repeat (match goal with
+       | [H1: Invariant.inject_value ?inv ?vt1 ?vt2 = true |- _] =>
+         exploit InvState.Rel.inject_value_spec; try exact H1; eauto; clear H1
+       end;
+       (try by
+           match goal with
+           | [H: getOperandValue (CurTargetData ?conf) ?v (Locals (EC ?st)) (Globals ?conf) = Some ?gv1 |-
+              InvState.Unary.sem_valueT ?conf ?st ?invst (ValueT.lift Tag.physical ?v) = Some ?gv2] =>
+             destruct v; [ss; unfold IdT.lift; solve_sem_idT; eauto | ss]
+           end); i; des).
+
+Ltac inv_conf :=
+  match goal with
+  | [H: InvState.valid_conf _ _ ?conf_src ?conf_tgt |- _] =>
+    let TD := fresh in
+    let GL := fresh in
+    destruct H as [[TD GL]]; rewrite TD in *; rewrite GL in *
+  end.
+
+Lemma inject_mem_change
+      m_src conf_src cmd_src mc_src st0_src
+      m_tgt conf_tgt cmd_tgt mc_tgt st0_tgt
+      inv0 invmem0 invst0
+      (CONF: InvState.valid_conf m_src m_tgt conf_src conf_tgt)
+      (STATE : InvState.Rel.sem conf_src conf_tgt st0_src st0_tgt invst0 invmem0 inv0)
+      (MEM : InvMem.Rel.sem conf_src conf_tgt st0_src.(Mem) st0_tgt.(Mem) invmem0)
+      (INJECT_EVENT : postcond_cmd_inject_event cmd_src cmd_tgt inv0)
+      (MC_SRC : mem_change_of_cmd conf_src cmd_src st0_src.(EC).(Locals) = Some mc_src)
+      (MC_TGT : mem_change_of_cmd conf_tgt cmd_tgt st0_tgt.(EC).(Locals) = Some mc_tgt)
+  : mem_change_inject conf_src conf_tgt invmem0 mc_src mc_tgt.
+Proof.
+  destruct cmd_src; destruct cmd_tgt; ss; clarify;
+    (try by simtac; econs); (* cases including none *)
+    try by simtac;
+    unfold is_true in *;
+    repeat (des_bool; des);
+    inject_clarify;
+    exploit_inject_value;
+    inv_conf;
+    inject_clarify;
+    econs; eauto.
+  unfold Invariant.is_private in *. des_ifs.
+  destruct x as [t x]; unfold ValueT.lift in *. des_ifs.
+  inv STATE. inv SRC.
+  exploit PRIVATE.
+  { apply IdTSet.mem_2; eauto. }
+  { inv_conf. inject_clarify. }
+  i. des_ifs.
+  econs; eauto.
+Qed.
+
+(* lemmas for malloc *)
+Lemma malloc_result
       TD mem mem' sz gn a mb
       (MALLOC: malloc TD mem sz gn a = Some (mem', mb))
   : <<ALLOC_BLOCK: mb = mem.(Memory.Mem.nextblock)>> /\
@@ -403,22 +428,123 @@ Proof.
   des_ifs.
 Qed.
 
-Lemma inject_mem_change
-      conf_src cmd_src mc_src st0_src
-      conf_tgt cmd_tgt mc_tgt st0_tgt
-      inv0 invmem0 invst0
-      (STATE : InvState.Rel.sem conf_src conf_tgt st0_src st0_tgt invst0 invmem0 inv0)
-      (INJECT_EVENT : postcond_cmd_inject_event cmd_src cmd_tgt inv0)
-      (MC_SRC : mem_change_of_cmd conf_src cmd_src st0_src.(EC).(Locals) = Some mc_src)
-      (MC_TGT : mem_change_of_cmd conf_tgt cmd_tgt st0_tgt.(EC).(Locals) = Some mc_tgt)
-  : mem_change_inject conf_src conf_tgt invmem0 mc_src mc_tgt.
+Lemma valid_access_malloc_same
+      TD mem0 mem1 bsz gn a mb p chunk ofs
+      (MALLOC: malloc TD mem0 bsz gn a = Some (mem1, mb))
+      (OFS: 0 <= ofs /\
+               ofs + Memdata.size_chunk chunk <=
+               Size.to_Z bsz *
+               (get_or_else (GV2int TD Size.ThirtyTwo gn) 0) /\
+               (Memdata.align_chunk chunk | ofs))
+  : Memory.Mem.valid_access mem1 chunk mb ofs p.
 Proof.
+  unfold malloc in *.
+  des_ifs; des; ss.
+  - eapply Memory.Mem.valid_access_implies;
+      try apply Memtype.perm_F_any.
+    eapply Memory.Mem.valid_access_alloc_same; eauto.
+  - rewrite Z.mul_0_r in *.
+    specialize (Memdata.size_chunk_pos chunk). i.
+    omega.
+Qed.
+
+Lemma valid_access_malloc_inv
+      TD mem0 mem1 bsz gn a b mb p chunk ofs
+      (MALLOC: malloc TD mem0 bsz gn a = Some (mem1, mb))
+      (VALID: Memory.Mem.valid_access mem1 chunk b ofs p)
+  : if Values.eq_block b mb
+    then 0 <= ofs /\
+         ofs + Memdata.size_chunk chunk <=
+         Size.to_Z bsz * get_or_else (GV2int TD Size.ThirtyTwo gn) 0 /\
+         (Memdata.align_chunk chunk | ofs)
+    else Memory.Mem.valid_access mem0 chunk b ofs p.
+Proof.
+  unfold malloc in *.
+  exploit Memory.Mem.valid_access_alloc_inv; eauto.
+  des_ifs. ss. rewrite Z.mul_0_r in *. eauto.
+Qed.
+
+Lemma valid_access_malloc_other
+      TD mem0 bsz gn a mem1 mb b' ofs p chunk
+      (MALLOC: malloc TD mem0 bsz gn a = Some (mem1, mb))
+      (VALID: Memory.Mem.valid_access mem0 chunk b' ofs p)
+  : Memory.Mem.valid_access mem1 chunk b' ofs p.
+Proof.
+  unfold malloc in *.
+  apply some_injective in MALLOC.
+  eapply Memory.Mem.valid_access_alloc_other; eauto.
+Qed.
+
+Ltac clarify_malloc :=
+  unfold malloc in *;
+  repeat match goal with
+         | [H: Some (Memory.Mem.alloc _ _ _) = Some (_, _) |- _] =>
+           apply some_injective in H
+         | [H: Some (_, _) = Some (Memory.Mem.alloc _ _ _) |- _] =>
+           apply some_injective in H
+         end.
+
+Lemma malloc_contents_same
+      TD mem0 mem1 gsz gn a
+      mb ofs
+      (MALLOC: malloc TD mem0 gsz gn a = Some (mem1, mb))
+  : Maps.ZMap.get ofs (Maps.PMap.get mb (Memory.Mem.mem_contents mem1)) = Memdata.Undef.
+Proof.
+  clarify_malloc.
+  erewrite <- Memory.Mem.alloc_mem_contents; eauto.
+  rewrite (Memory.Mem.alloc_result _ _ _ _ _ MALLOC).
+  rewrite Maps.PMap.gss.
+  apply Maps.ZMap.gi.
+Qed.
+
+Lemma malloc_contents_other
+      TD mem0 mem1 gsz gn a
+      mb b ofs
+      (MALLOC: malloc TD mem0 gsz gn a = Some (mem1, mb))
+      (DIFF: b <> mb)
+  : Maps.ZMap.get ofs (Maps.PMap.get b (Memory.Mem.mem_contents mem1)) =
+    Maps.ZMap.get ofs (Maps.PMap.get b (Memory.Mem.mem_contents mem0)).
+Proof.
+  clarify_malloc.
+  erewrite <- Memory.Mem.alloc_mem_contents; eauto.
+  rewrite (Memory.Mem.alloc_result _ _ _ _ _ MALLOC) in DIFF.
+  rewrite Maps.PMap.gsspec.
+  des_ifs.
+Qed.
+
+(* end of malloc *)
+
+Lemma invmem_unary_src_alloc_preserved
+      conf invmem0 mem0 mem1
+      public gmax mb
+      gsz gn a
+      (SRC : InvMem.Unary.sem conf gmax public mem0 invmem0)
+      (MALLOC : Some (mem1, mb) = malloc (CurTargetData conf) mem0 gsz gn a)
+  : InvMem.Unary.sem conf gmax public mem1 invmem0.
+Proof.
+  exploit malloc_result; eauto. i. des.
+  inv SRC.
+  econs; eauto.
+  - i. exploit PRIVATE; eauto. i. des.
+    split; eauto.
+    eapply Pos.lt_trans; eauto.
+    rewrite NEXT_BLOCK. apply Plt_succ'.
+  - i. exploit PRIVATE_PARENT; eauto. i. des.
+    split; eauto.
+    eapply Pos.lt_trans; eauto.
+    rewrite NEXT_BLOCK. apply Plt_succ'.
+  - i. exploit MEM_PARENT; eauto. i.
+    rewrite x.
+    admit. (* We can deduce b <> (mem0.nextblock) so mload_aux is preserved *)
 Admitted.
 
+(* TODO: simplify proof script *)
+
 Lemma inject_invmem
-      conf_src st0_src st1_src cmd_src cmds_src evt_src
-      conf_tgt st0_tgt st1_tgt cmd_tgt cmds_tgt evt_tgt
+      m_src conf_src st0_src st1_src cmd_src cmds_src evt_src
+      m_tgt conf_tgt st0_tgt st1_tgt cmd_tgt cmds_tgt evt_tgt
       invst0 invmem0 inv0 inv1
+      (CONF: InvState.valid_conf m_src m_tgt conf_src conf_tgt)
       (STATE : InvState.Rel.sem conf_src conf_tgt st0_src st0_tgt invst0 invmem0 inv0)
       (MEM : InvMem.Rel.sem conf_src conf_tgt (Mem st0_src) (Mem st0_tgt) invmem0)
       (CMD_SRC : CurCmds (EC st0_src) = cmd_src :: cmds_src)
@@ -435,7 +561,619 @@ Lemma inject_invmem
     <<MEM: InvMem.Rel.sem conf_src conf_tgt (Mem st1_src) (Mem st1_tgt) invmem1 >> /\
     <<MEMLE: InvMem.Rel.le invmem0 invmem1 >>.
 Proof.
-  (* TODO: mc ~ mc0 *)
+  hexploit step_mem_change; try (inv STATE; exact SRC); eauto. intro MCS. destruct MCS as [mc_src [MC_SOME_SRC [MC_AFTER_SRC STATE_EQUIV_SRC]]]. des.
+  hexploit step_mem_change; try (inv STATE; exact TGT); eauto. intro MCS. destruct MCS as [mc_tgt [MC_SOME_TGT [MC_AFTER_TGT STATE_EQUIV_TGT]]]. des.
+
+  exploit inject_mem_change; eauto. intro MC_INJECT.
+
+  inv MC_INJECT.
+  - (* alloc - alloc *)
+    inv STEP_SRC; inv CMD_SRC; ss; try by des; congruence.
+    rename Mem0 into mem0_src. rename Mem' into mem1_src. rename mb into mb_src.
+    match goal with
+    | [H: malloc _ _ _ _ _ = _ |- _] => rename H into MALLOC_SRC
+    end.
+    inv STEP_TGT; inv CMD_TGT; ss; try by des; congruence.
+    rename Mem0 into mem0_tgt. rename Mem' into mem1_tgt. rename mb into mb_tgt.
+    match goal with
+    | [H: malloc _ _ _ _ _ = _ |- _] => rename H into MALLOC_TGT
+    end.
+    eexists.
+    instantiate (1:= InvMem.Rel.mk _ _ _ (fun b => if Values.eq_block b mb_src then Some (mb_tgt, 0%Z) else invmem0.(InvMem.Rel.inject) b)).
+    esplits.
+    + (* alloc_inject *)
+      ii. ss.
+      inv ALLOCA_SRC. inv ALLOCA_TGT.
+      esplits; try apply lookupAL_updateAddAL_eq; ss.
+      destruct (Values.eq_block mb_src mb_src); ss.
+    + (* InvMem sem *)
+      inv MEM; ss.
+      econs; ss; eauto.
+      { (* SRC *)
+        inv SRC.
+        hexploit (@malloc_result TD mem0_src); eauto. i. des.
+        econs; eauto.
+        { 
+          i. exploit PRIVATE; eauto. i.
+          des.
+          destruct (Values.eq_block b mb_src) eqn:EQ_MB.
+          - subst.
+            exploit Pos.lt_irrefl; eauto. contradiction.
+          - split.
+            + ii.
+              match goal with
+              | [H: ~ InvMem.Rel.public_src _ _ |- False] =>
+                apply H
+              end.
+              unfold InvMem.Rel.public_src in *. rewrite EQ_MB in *. eauto.
+            + eapply Pos.lt_trans; eauto.
+              apply Pos.le_succ_l. rewrite NEXT_BLOCK. apply Pos.le_refl.
+        }
+        { i. exploit PRIVATE_PARENT; eauto. i. des.
+          destruct (Values.eq_block b mb_src) eqn:EQ_MB.
+          - subst.
+            exploit Pos.lt_irrefl; eauto. contradiction.
+          - split.
+            + ii. apply x.
+              unfold InvMem.Rel.public_src in *. rewrite EQ_MB in *. eauto.
+            + eapply Pos.lt_trans; eauto.
+              apply Pos.le_succ_l. rewrite NEXT_BLOCK. apply Pos.le_refl.
+        }
+        { i. exploit MEM_PARENT; eauto. i.
+          match goal with
+          | [H: mload_aux (InvMem.Unary.mem_parent _) _ b _ = _ |- _] =>
+            rewrite H
+          end.
+          exploit PRIVATE_PARENT; eauto. i. des.
+          admit. (* b is less than Mem0's nextblock, and Mem0 -alloc-> Mem' so mload_aux is preserved *)
+        }
+      }
+      { (* TGT *)
+        inv TGT.
+        hexploit (@malloc_result TD0 mem0_tgt); eauto. i. des.
+        econs; eauto.
+        { 
+          i. exploit PRIVATE; eauto. i.
+          des.
+          split.
+          { ii.
+            match goal with
+            | [H: ~ InvMem.Rel.public_tgt _ _ |- False] =>
+              apply H
+            end.
+            unfold InvMem.Rel.public_tgt in *. des.
+            destruct (Values.eq_block b_src mb_src).
+            { clarify. exfalso. eapply Pos.lt_irrefl; eauto. }
+            { esplits; eauto. }
+          }
+          { eapply Pos.lt_trans; eauto.
+            apply Pos.le_succ_l. rewrite NEXT_BLOCK. apply Pos.le_refl.
+          }
+        }
+        { i. exploit PRIVATE_PARENT; eauto. i. des.
+          split.
+          { ii.
+            match goal with
+            | [H: ~ InvMem.Rel.public_tgt _ _ |- False] =>
+              apply H
+            end.
+            unfold InvMem.Rel.public_tgt in *. des.
+            destruct (Values.eq_block b_src mb_src).
+            { clarify. exfalso. eapply Pos.lt_irrefl; eauto. }
+            { esplits; eauto. }
+          }
+          { eapply Pos.lt_trans; eauto.
+            apply Pos.le_succ_l. rewrite NEXT_BLOCK. apply Pos.le_refl.
+          }
+        }
+        { i. exploit MEM_PARENT; eauto. i.
+          match goal with
+          | [H: mload_aux (InvMem.Unary.mem_parent _) _ b _ = _ |- _] =>
+            rewrite H
+          end.
+          exploit PRIVATE_PARENT; eauto. i. des.
+          admit. (* b is less than Mem0's nextblock, and Mem0 -alloc-> Mem' so mload_aux is preserved *)
+        }
+      }
+      { (* inject *)
+        inv INJECT.
+        unfold is_true in *.
+        repeat rewrite andb_true_iff in INJECT_EVENT.
+        destruct INJECT_EVENT as [[[ID_EQ TYP_EQ] INJECT_VALUE] DEC_EQ].
+        unfold proj_sumbool in *. des_ifs.
+        econs.
+        { (* mi_access *)
+          ii. exploit valid_access_malloc_inv; try exact MALLOC_SRC; eauto. i.
+          destruct (Values.eq_block b1 mb_src).
+          { clarify.
+            eapply valid_access_malloc_same; eauto.
+            admit. (* gn >= gn2 *)
+          }
+          { exploit mi_access; eauto.
+            eapply valid_access_malloc_other; eauto.
+          }
+        }
+        { (* mi_memval *)
+          i. destruct (Values.eq_block b1 mb_src).
+          - clarify.
+            rewrite Z.add_0_r.
+            erewrite malloc_contents_same; eauto.
+            erewrite malloc_contents_same; eauto.
+            apply memory_sim.MoreMem.memval_inject_undef.
+          - eapply memory_sim.MoreMem.memval_inject_incr.
+            { assert (DIFF_BLK_TGT: b2 <> mb_tgt).
+              { exploit genericvalues_inject.Hmap2; eauto. i.
+                exploit (Memory.Mem.alloc_result mem0_tgt); eauto.
+                { clarify_malloc. eauto. }
+                ii. subst.
+                eapply Pos.lt_irrefl. eauto.
+              }
+              eapply malloc_contents_other in DIFF_BLK_TGT; eauto.
+              rewrite DIFF_BLK_TGT.
+              erewrite malloc_contents_other; eauto.
+              apply mi_memval; eauto.
+              exploit Memory.Mem.perm_alloc_inv.
+              { clarify_malloc. exact MALLOC_SRC. }
+              { eauto. }
+              i. des_ifs.
+            }
+            { ii.
+              destruct (Values.eq_block b mb_src).
+              { subst. exfalso.
+                exploit genericvalues_inject.Hmap1; eauto.
+                { instantiate (1:=mb_src).
+                  clarify_malloc.
+                  exploit (Memory.Mem.alloc_result mem0_src); eauto. i.
+                  subst. apply Pos.le_ge. apply Pos.le_refl. }
+                i. congruence.
+              }
+              eauto.
+            }
+        }
+      }
+      { (* wf_sb_mi *)
+        inv WF.
+        exploit malloc_result; try exact MALLOC_SRC. intros [ALLOC_BLOCK_SRC NEXT_BLOCK_SRC]. des.
+        exploit malloc_result; try exact MALLOC_TGT. intros [ALLOC_BLOCK_TGT NEXT_BLOCK_TGT]. des.
+        econs.
+        - (* no_overlap *)
+          ii.
+          destruct (Values.eq_block b1 mb_src);
+            destruct (Values.eq_block b2 mb_src); clarify.
+          + exploit Hmap2; eauto. i.
+            eapply Pos.lt_irrefl; eauto.
+          + exploit Hmap2; eauto. i.
+            eapply Pos.lt_irrefl; eauto.
+          + eapply Hno_overlap with (b1:=b1) (b2:=b2); eauto.
+        - (* destruct (Values.eq_block Memory.Mem.nullptr mb_src). *)
+          (* - subst. *)
+          (*   hexploit Memory.Mem.alloc_result. *)
+          (*   { clarify_malloc. exact MALLOC_SRC. } *)
+          (*   i. *)
+          (* - done. *)
+          admit. (* nullptr will be removed *)
+        - (* Hmap1 *)
+          i. destruct (Values.eq_block b mb_src).
+          + subst.
+            rewrite NEXT_BLOCK_SRC in *.
+            exfalso.
+            eapply Pos.lt_nle.
+            { apply Plt_succ'. }
+            apply Pos.ge_le.
+            eauto.
+          + apply Hmap1.
+            apply Pos.le_ge.
+            eapply Pos.le_trans.
+            { apply Ple_succ. }
+            { rewrite NEXT_BLOCK_SRC in *.
+              apply Pos.ge_le. eauto.
+            }
+        - (* Hmap2 *)
+          i. destruct (Values.eq_block b1 mb_src).
+          + clarify.
+            subst. rewrite NEXT_BLOCK_TGT in *.
+            apply Plt_succ'.
+          + exploit Hmap2; eauto. i.
+            eapply Pos.lt_trans; eauto.
+            rewrite NEXT_BLOCK_TGT.
+            apply Plt_succ'.
+        - (* mi_freeblocks *)
+          intros b NOT_VALID_BLOCK.
+          destruct (Values.eq_block b mb_src).
+          + subst.
+            exfalso.
+            apply NOT_VALID_BLOCK.
+            unfold Memory.Mem.valid_block.
+            rewrite NEXT_BLOCK_SRC.
+            eapply Plt_succ'.
+          + apply mi_freeblocks. intros VALID_BLOCK.
+            apply NOT_VALID_BLOCK.
+            unfold Memory.Mem.valid_block in *.
+            rewrite NEXT_BLOCK_SRC.
+            eapply Pos.lt_trans; eauto.
+            apply Plt_succ'.
+        - (* mi_mappedblocks *)
+          i. destruct (Values.eq_block b mb_src).
+          + clarify.
+            unfold Memory.Mem.valid_block in *.
+            rewrite NEXT_BLOCK_TGT.
+            apply Plt_succ'.
+          + eapply Memory.Mem.valid_block_alloc.
+            { clarify_malloc. eauto. }
+            eapply mi_mappedblocks; eauto.
+        - (* mi_range_blocks *)
+          ii. destruct (Values.eq_block b mb_src).
+          + subst. clarify.
+          + eapply mi_range_block; eauto.
+        - (* mi_bounds *)
+          ii. destruct (Values.eq_block b mb_src).
+          + clarify.
+            erewrite Memory.Mem.bounds_alloc_same; cycle 1.
+            { clarify_malloc. exact MALLOC_SRC. }
+            erewrite Memory.Mem.bounds_alloc_same; cycle 1.
+            { clarify_malloc. exact MALLOC_TGT. }
+            apply injective_projections; ss.
+            admit. (* GV2int returns 0 => malloc 0-sized space *)
+          + erewrite Memory.Mem.bounds_alloc_other with (b':=b); eauto; cycle 1.
+            { clarify_malloc. exact MALLOC_SRC. }
+            assert (NEQ_BLK_TGT: b' <> mb_tgt).
+            { exploit Hmap2; eauto. ii. subst.
+              eapply Plt_irrefl. eauto. }
+            erewrite Memory.Mem.bounds_alloc_other with (b':=b'); try exact NEQ_BLK_TGT; cycle 1.
+            { clarify_malloc. exact MALLOC_TGT. }
+            eapply mi_bounds; eauto.
+        - (* mi_globals *)
+          i. destruct (Values.eq_block b mb_src).
+          + subst.
+            exploit mi_globals; eauto. i.
+            exploit Hmap1.
+            { apply Pos.le_ge.
+              apply Pos.le_refl.
+            }
+            i. congruence.
+          + exploit mi_globals; eauto.
+      }
+    + (* le *)
+      econs; try (econs; ss).
+      (* incr *)
+      ii. ss.
+      exploit malloc_result; try exact MALLOC_SRC. intros [ALLOC_BLOCK_SRC NEXT_BLOCK_SRC]. des.
+      exploit malloc_result; try exact MALLOC_TGT. intros [ALLOC_BLOCK_TGT NEXT_BLOCK_TGT]. des.
+      destruct (Values.eq_block b mb_src); eauto.
+      subst.
+      inv MEM. inv WF.
+      exploit Hmap1.
+      { apply Pos.le_ge. apply Pos.le_refl. }
+      i. congruence.
+  - (* alloc - none *)
+    esplits; eauto.
+    + ii.
+      Ltac solve_alloc_inject :=
+        match goal with
+        | [ALLOCA: ?cmd = insn_alloca _ _ _ _,
+                 MC_SOME: mem_change_of_cmd _ ?cmd _ = Some mem_change_none |- _] =>
+          rewrite ALLOCA in MC_SOME; ss; des_ifs
+        end.
+      solve_alloc_inject.
+    + inv MEM.
+      inv STATE_EQUIV_TGT. rewrite <- MEM_EQ in *.
+      inv STATE_EQUIV_SRC.
+      econs; eauto.
+      * eapply invmem_unary_src_alloc_preserved; eauto.
+      * inv INJECT.
+        econs.
+        { (* mi-access *)
+          i. exploit mi_access; eauto.
+          (* we can deduce b1 is less than nextblock *)
+          (* then valid_access_malloc_inv trivially solves the problem *)
+          admit.
+        }
+        { (* mi_memval *)
+          i. exploit mi_memval; eauto.
+          { (* use Memory.Mem.perm_alloc_inv *)
+            admit. }
+          i. (* b1 is less then nextblock *)
+          exploit malloc_contents_other; eauto.
+          { admit. }
+          intro CONTENTS.
+          rewrite CONTENTS. eauto.
+        }
+      * inv WF.
+        econs; eauto.
+        { (* Hmap1 *)
+          (* b >= nextblock mem1 >= nextblock mem0 *)
+          admit. }
+        { (* same *)
+          admit. }
+        { (* b >= nextblock, so bounds preserved *)
+          (* Memory.Mem.bounds_alloc *)
+          admit. }
+    + reflexivity.
+  - (* none - alloc *)
+    admit.
+  - (* store - store *)
+    admit.
+  - (* store - none *)
+    admit.
+  - (* free - free *)
+    admit.
+  - (* none - none *)
+    admit.
+Admitted.
+
+(* We use this as an axiom for now *)
+Lemma mstore_noalias_mload
+      conf mem0 mem1 TD
+      sptr sty gv sa
+      lptr lty la
+      (STORE: Some mem1 = mstore TD mem0 sptr sty gv sa)
+      (NOALIAS: InvState.Unary.sem_noalias conf sptr lptr sty lty)
+  : mload TD mem1 lptr lty la = mload TD mem0 lptr lty la.
+Proof.
+Admitted.
+
+Lemma diffblock_comm
+      conf gv1 gv2
+      (DIFFBLOCK: InvState.Unary.sem_diffblock conf gv1 gv2)
+  : InvState.Unary.sem_diffblock conf gv2 gv1.
+Proof.
+  unfold InvState.Unary.sem_diffblock in *. des_ifs. eauto.
+Qed.
+
+Lemma noalias_comm
+      conf gv1 gv2 ty1 ty2
+      (NOALIAS: InvState.Unary.sem_noalias conf gv1 gv2 ty1 ty2)
+  : InvState.Unary.sem_noalias conf gv2 gv1 ty2 ty1.
+Proof.
+  unfold InvState.Unary.sem_noalias in *. des_ifs. eauto.
+Qed.  
+
+Lemma diffblock_implies_noalias
+      conf gv1 gv2 ty1 ty2
+      (DIFFBLOCK: InvState.Unary.sem_diffblock conf gv1 gv2)
+  : InvState.Unary.sem_noalias conf gv1 gv2 ty1 ty2.
+Proof.
+  unfold InvState.Unary.sem_diffblock, InvState.Unary.sem_noalias in *. des_ifs.
+Qed.
+
+(* TODO: prove this after adding unique<>globals*)
+Lemma const_unique_diffblock
+      conf c gv_c
+      st1 x_inv gv_inv val
+      (FORGET_PTR : const2GV (CurTargetData conf) (Globals conf) c = Some gv_c)
+      (VAL : lookupAL GenericValue (Locals (EC st1)) x_inv = Some gv_inv)
+      (XX : forall (gid : atom) (gptr : GenericValue),
+          lookupAL GenericValue (Globals conf) gid = Some gptr -> InvState.Unary.sem_diffblock conf val gptr)
+  : InvState.Unary.sem_diffblock conf gv_c gv_inv.
+Proof.
+(* destruct c. *)
+(* - unfold InvState.Unary.sem_diffblock. *)
+(*   des_ifs. *)
+(*   unfold const2GV in *. des_ifs. *)
+(*   unfold _const2GV in *. des_ifs. *)
+(*   unfold zeroconst2GV in *. des_ifs. ss. *)
+(*   unfold zeroconst2GV_aux in *. *)
+(*   unfold GV2ptr in *. des_ifs. *)
+Admitted.
+
+Lemma is_diffblock_sem
+      conf st invst invmem inv
+      v1 ty1 v2 ty2 gv1 gv2
+      (STATE : InvState.Unary.sem conf st invst invmem inv)
+      (IS_DIFFBLOCK : Invariant.is_diffblock inv (v1, ty1) (v2, ty2) = true)
+      (VAL1 : InvState.Unary.sem_valueT conf st invst v1 = Some gv1)
+      (VAL2 : InvState.Unary.sem_valueT conf st invst v2 = Some gv2)
+  : InvState.Unary.sem_diffblock conf gv1 gv2.
+Proof.
+  inv STATE.
+  destruct NOALIAS as [DIFFBLOCK NOALIAS].
+  unfold Invariant.is_diffblock in *.
+  unfold flip in *.
+  apply ValueTPairSetFacts.exists_iff in IS_DIFFBLOCK; try by solve_compat_bool.
+  inv IS_DIFFBLOCK.
+  destruct x as [p1 p2].
+  des. des_bool. des.
+  - des_bool. des. ss.
+    unfold proj_sumbool in *; des_ifs.
+    rewrite ValueTPairSetFacts.mem_iff in *.
+    exploit DIFFBLOCK; eauto.
+  - des_bool. des. ss.
+    unfold proj_sumbool in *; des_ifs.
+    rewrite ValueTPairSetFacts.mem_iff in *.
+    exploit DIFFBLOCK; eauto.
+    apply diffblock_comm.
+Qed.
+
+Lemma is_noalias_sem
+      conf st invst invmem inv
+      v1 ty1 v2 ty2 gv1 gv2
+      (STATE : InvState.Unary.sem conf st invst invmem inv)
+      (IS_NOALIAS : Invariant.is_noalias inv (v1, ty1) (v2, ty2) = true)
+      (VAL1 : InvState.Unary.sem_valueT conf st invst v1 = Some gv1)
+      (VAL2 : InvState.Unary.sem_valueT conf st invst v2 = Some gv2)
+  : InvState.Unary.sem_noalias conf gv1 gv2 ty1 ty2.
+Proof.
+  inv STATE.
+  destruct NOALIAS as [DIFFBLOCK NOALIAS].
+  unfold Invariant.is_noalias in *.
+  unfold flip in *.
+  apply PtrPairSetFacts.exists_iff in IS_NOALIAS; try by solve_compat_bool.
+  inv IS_NOALIAS.
+  destruct x as [p1 p2].
+  Opaque PtrSetFacts.eq_dec.
+  unfold proj_sumbool in *.
+  des. des_bool. des.
+  - des_bool. des. ss. des_ifs.
+    rewrite PtrPairSetFacts.mem_iff in *.
+    exploit NOALIAS; subst; eauto.
+  - des_bool. des. ss. des_ifs.
+    rewrite PtrPairSetFacts.mem_iff in *.
+    exploit NOALIAS; subst; eauto.
+    apply noalias_comm.
+Qed.
+
+(* TODO: simplify proof script *)
+Lemma forget_memory_is_noalias_expr
+      conf st1 invst0 invmem0 inv1 mem0
+      vt_inv ty_inv gv_inv
+      v_forget ty_forget gv_forget
+      (STATE : InvState.Unary.sem conf (mkState st1.(EC) st1.(ECS) mem0) invst0 invmem0 inv1)
+      (NOALIAS_PTR: ForgetMemory.is_noalias_Ptr inv1 (ValueT.lift Tag.physical v_forget, ty_forget) (vt_inv, ty_inv) = true)
+      (FORGET_PTR: getOperandValue (CurTargetData conf) v_forget (Locals (EC st1)) (Globals conf) = Some gv_forget)
+      (INV_PTR: InvState.Unary.sem_valueT conf st1 invst0 vt_inv = Some gv_inv)
+  : InvState.Unary.sem_noalias conf gv_forget gv_inv ty_forget ty_inv.
+Proof.
+  unfold ForgetMemory.is_noalias_Ptr in *.
+  do 4 (des_bool; des).
+  - rename NOALIAS_PTR0 into DIFFBLOCK_FROM_UNIQUE.
+    des_bool. des. des_bool.
+    rename NOALIAS_PTR0 into INV_UNIQUE.
+    unfold proj_sumbool in *. des_ifs. ss.
+
+    unfold Invariant.is_unique_ptr in *.
+    unfold Invariant.is_unique_value in *.
+    unfold proj_sumbool in *.
+    ss. des_ifs. des_bool. des.
+    destruct x as [[] x_inv]; ss.
+
+    inv STATE.
+    exploit UNIQUE; eauto.
+    { apply AtomSetFacts.mem_iff; eauto. }
+    intro UNIQUE_X. inv UNIQUE_X.
+
+    unfold Invariant.values_diffblock_from_unique in *.
+    destruct v_forget as [x_forget| c_forget]; ss.
+    + assert (IDS_NEQ: x_forget <> x_inv).
+      { unfold IdT.lift in *.
+        match goal with
+        | [H: _ <> _ |- _] =>
+          ii; subst; apply H; reflexivity
+        end. }
+      apply diffblock_implies_noalias.
+      unfold InvState.Unary.sem_idT in *. ss. clarify.
+      apply diffblock_comm.
+      
+      eapply LOCALS; eauto.
+    + assert (XX:
+                forall gid gptr,
+                  lookupAL _ conf.(Globals) gid = Some gptr ->
+                  InvState.Unary.sem_diffblock conf val gptr).
+      { admit. (* sem_unique seems to have to guarantee this *) }
+      apply diffblock_implies_noalias.
+      unfold InvState.Unary.sem_idT in *. ss. clarify.
+      eapply const_unique_diffblock; eauto.
+  - rename NOALIAS_PTR0 into DIFFBLOCK_FROM_UNIQUE.
+    des_bool. des. des_bool.
+    rename NOALIAS_PTR0 into INV_UNIQUE.
+    unfold proj_sumbool in *. des_ifs. ss.
+
+    unfold Invariant.is_unique_ptr in *.
+    unfold Invariant.is_unique_value in *.
+    unfold proj_sumbool in *.
+    ss. des_ifs. des_bool. des.
+
+    destruct x as [[] x_forget]; ss.
+    destruct v_forget; ss.
+    clarify.
+
+    inv STATE.
+    exploit UNIQUE; eauto.
+    { apply AtomSetFacts.mem_iff; eauto. }
+    intro UNIQUE_X. inv UNIQUE_X.
+
+    unfold Invariant.values_diffblock_from_unique in *.
+    destruct vt_inv as [[[] x_inv]| c_inv]; ss.
+    + assert (IDS_NEQ: x_forget <> x_inv).
+      { unfold IdT.lift in *.
+        match goal with
+        | [H: _ <> _ |- _] =>
+          ii; subst; apply H; reflexivity
+        end. }
+      apply diffblock_implies_noalias.
+      unfold InvState.Unary.sem_idT in *. ss. clarify.
+      
+      eapply LOCALS; eauto.
+    + assert (XX:
+                forall gid gptr,
+                  lookupAL _ conf.(Globals) gid = Some gptr ->
+                  InvState.Unary.sem_diffblock conf val gptr).
+      { admit. (* sem_unique seems to have to guarantee this *) }
+      apply diffblock_implies_noalias.
+      apply diffblock_comm.
+      unfold InvState.Unary.sem_idT in *. ss. clarify.
+      eapply const_unique_diffblock; eauto.
+  - exploit is_noalias_sem.
+    { eauto. }
+    { eauto. }
+    { eauto. }
+    { unfold ValueT.lift. des_ifs; eauto. }
+    i. apply noalias_comm. eauto.
+  - exploit is_diffblock_sem.
+    { eauto. }
+    { eauto. }
+    { eauto. }
+    { destruct v_forget as [x_forget|c_forget]; eauto. }
+    i. apply diffblock_implies_noalias.
+    apply diffblock_comm. eauto.
+Admitted.
+
+Lemma forget_memory_is_noalias_exprpair
+      conf st1 invst0 invmem0 inv1 mem0
+      p a e2
+      vt_inv ty_inv gv_inv
+      v_forget ty_forget gv_forget
+      (STATE : InvState.Unary.sem conf (mkState st1.(EC) st1.(ECS) mem0) invst0 invmem0 inv1)
+      (PAIR : p = (Expr.load vt_inv ty_inv a, e2) \/ p = (e2, Expr.load vt_inv ty_inv a))
+      (FORGET_MEMORY_IN : ExprPairSet.In p (Invariant.lessdef inv1))
+      (FORGET_MEMORY_NOALIAS : ForgetMemory.is_noalias_ExprPair inv1 (ValueT.lift Tag.physical v_forget, ty_forget) p = true)
+      (FORGET_PTR: getOperandValue (CurTargetData conf) v_forget (Locals (EC st1)) (Globals conf) = Some gv_forget)
+      (INV_PTR: InvState.Unary.sem_valueT conf st1 invst0 vt_inv = Some gv_inv)
+  : InvState.Unary.sem_noalias conf gv_forget gv_inv ty_forget ty_inv.
+Proof.
+  unfold ForgetMemory.is_noalias_ExprPair in *.
+  des; des_bool; des; subst; ss;
+    eapply forget_memory_is_noalias_expr; eauto.
+Qed.
+
+Lemma exprpair_forget_memory_disjoint
+      conf st1 mem0 invst0 invmem0 inv1
+      cmd mc ptr
+      p e1 e2
+      (STATE: InvState.Unary.sem conf (mkState st1.(EC) st1.(ECS) mem0) invst0 invmem0 inv1)
+      (* (UNIQUE: AtomSetImpl.For_all (InvState.Unary.sem_unique conf (mkState st1.(EC) st1.(ECS) mem0)) *)
+      (*                                                         (Invariant.unique inv1)) *)
+      (MC_SOME : mem_change_of_cmd conf cmd st1.(EC).(Locals) = Some mc)
+      (STATE_EQUIV : states_mem_change conf mem0 st1.(Mem) mc)
+      (DEF_MEMORY: Cmd.get_def_memory cmd = Some ptr)
+      (PAIR: p = (e1, e2) \/ p = (e2, e1))
+      (FORGET_MEMORY : ExprPairSet.In p
+                                      (Invariant.lessdef
+                                         (ForgetMemory.unary ptr inv1)))
+  : InvState.Unary.sem_expr conf st1 invst0 e1 =
+    InvState.Unary.sem_expr conf (mkState st1.(EC) st1.(ECS) mem0) invst0 e1.
+Proof.
+  destruct mc.
+  - (* alloc *)
+    destruct cmd; ss; des_ifs.
+  - (* store *)
+    destruct cmd; ss; des_ifs.
+    inv STATE_EQUIV.
+    destruct e1; ss.
+    + replace (InvState.Unary.sem_list_valueT conf {| EC := EC st1; ECS := ECS st1; Mem := mem0 |} invst0 lsv)
+              with (InvState.Unary.sem_list_valueT conf st1 invst0 lsv); ss.
+      clear.
+      induction lsv; ss.
+      destruct a. rewrite <- IHlsv. ss.
+    + erewrite sem_valueT_eq_locals with (st1:=mkState st1.(EC) st1.(ECS) mem0); [| ss].
+      des_ifs.
+      apply ExprPairSetFacts.filter_iff in FORGET_MEMORY; try by solve_compat_bool.
+      destruct FORGET_MEMORY as [FORGET_MEMORY_IN FORGET_MEMORY_NOALIAS].
+      eapply mstore_noalias_mload; eauto.
+      exploit forget_memory_is_noalias_exprpair; eauto.
+  - (* free *)
+    admit.
+  - (* none *)
+    inv STATE_EQUIV. destruct st1; eauto.
 Admitted.
 
 Lemma forget_memory_equiv_except_mem
@@ -453,6 +1191,13 @@ Lemma forget_memory_equiv_except_mem
   : InvState.Rel.sem conf_src conf_tgt st1_src st1_tgt invst0 invmem0
                      (ForgetMemory.t (Cmd.get_def_memory cmd_src) (Cmd.get_def_memory cmd_tgt) inv1).
 Proof.
+  (* inv STATE_FORGET. *)
+  (* econs. *)
+  (* { (* SRC *) *)
+  (*   inv SRC. *)
+  (*   econs. *)
+  (*   - ii. *)
+  
 Admitted.
 
 Lemma forget_memory_sound
@@ -487,22 +1232,11 @@ Lemma forget_memory_sound
       <<MEM: InvMem.Rel.sem conf_src conf_tgt st1_src.(Mem) st1_tgt.(Mem) invmem1>> /\
       <<MEMLE: InvMem.Rel.le invmem0 invmem1>>.
 Proof.
-  exploit step_mem_change.
-  { inv STATE. exact SRC. }
-  { eauto. }
-  { eauto. }
-  { eauto. }
-  { eauto. }
-  exploit step_mem_change.
-  { inv STATE. exact TGT. }
-  { eauto. }
-  { eauto. }
-  { eauto. }
-  { eauto. }
-  i. des.
-
-  exploit inject_invmem; try exact INJECT_EVENT; eauto.
-  i. des.
+  assert (STATE2:= STATE).
+  inv STATE2.
+  exploit step_mem_change; try exact SRC; eauto. i. des.
+  exploit step_mem_change; try exact TGT; eauto. i. des.
+  exploit inject_invmem; try exact INJECT_EVENT; eauto. i. des.
   esplits; eauto.
 
   eapply forget_memory_equiv_except_mem; eauto.
@@ -925,3 +1659,180 @@ Admitted.
 (* (*     hexploit mem_inject_change; try exact MEM_CHANGE_INJECT; eauto. i. *) *)
 (* (*     esplits; econs; eauto. *) *)
 (* (* Qed. *) *)
+
+
+
+
+(* from postcond cmd *)
+
+
+(* Lemma step_equiv_except_mem *)
+(*       conf st0 st1 evt *)
+(*       cmd cmds *)
+(*       invst0 invmem0 inv0 inv1 *)
+(*       public gmax *)
+(*       (STATE: InvState.Unary.sem conf st0 invst0 invmem0 inv0) *)
+(*       (MEM: InvMem.Unary.sem conf gmax public st0.(Mem) invmem0) *)
+(*       (NONCALL: Instruction.isCallInst cmd = false) *)
+(*       (CMDS: CurCmds st0.(EC) = cmd :: cmds) *)
+(*       (FORGET: inv_unary_forgot inv1 (AtomSetImpl_from_list (option_to_list (Cmd.get_def cmd)))) *)
+(*       (STEP: sInsn conf st0 st1 evt) *)
+(*   : exists mc, *)
+(*     <<MEM_CH_REL: mem_change_cmd conf st0 mc cmd>> /\ *)
+(*     <<STATE_EQUIV: state_equiv_except_mem conf (mkState st1.(EC) st1.(ECS) st0.(Mem)) st1 mc>>. *)
+(* Proof. *)
+(*   inv STEP; destruct cmd; inv CMDS; ss; *)
+(*     try by esplits; eauto; econs; eauto; econs; eauto. *)
+(*   - admit. (* malloc , should know newly allocated block is unique *) *)
+(*   - admit. (* alloca *) *)
+(* Admitted. *)
+
+(* Lemma step_unique_preserved_mem *)
+(*       conf st0 st1 evt *)
+(*       cmd cmds inv0 *)
+(*       (STATE: AtomSetImpl.For_all (InvState.Unary.sem_unique conf (mkState st1.(EC) st1.(ECS) st0.(Mem))) *)
+(*                                   inv0.(Invariant.unique)) *)
+(*       (NONCALL: Instruction.isCallInst cmd = false) *)
+(*       (CMDS: CurCmds st0.(EC) = cmd :: cmds) *)
+(*       (STEP: sInsn conf st0 st1 evt) *)
+(*       (UNIQUE_NOT_LEAKED: forall x (MEM:AtomSetImpl.mem x inv0.(Invariant.unique) = true), *)
+(*                                  AtomSetImpl.mem x (AtomSetImpl_from_list (Cmd.get_leaked_ids cmd)) = false) *)
+(*   : unique_preserved_mem conf st1 inv0. *)
+(* Proof. *)
+(*   inv STEP; ss; *)
+(*     try (inv CMDS; ss; *)
+(*          ii; specialize_unique; eauto). *)
+(*   { admit. (* load malloc -> undef *) } *)
+(*   { admit. (* load after free: use Memory.Mem.load_free_2 maybe *) } *)
+(*   { admit. (* load alloca *) } *)
+(*   { admit. (* load after store *) } *)
+(* Admitted. *)
+
+(* Lemma mem_change_cmd_state_transition *)
+(*       conf st0 st1 evt cmd cmds mc inv0 *)
+(*       (CMD: CurCmds (EC st0) = cmd :: cmds) *)
+(*       (NONCALL: Instruction.isCallInst cmd = false) *)
+(*       (STEP: sInsn conf st0 st1 evt) *)
+(*       (MEM_CH_REL: mem_change_cmd conf st0 mc cmd) *)
+(*       (FORGET: inv_unary_forgot inv0 (AtomSetImpl_from_list (option_to_list (Cmd.get_def cmd)))) *)
+(*   : mem_change_cmd_after conf {| EC := EC st1; ECS := ECS st1; Mem := Mem st0 |} mc cmd inv0. *)
+(* Proof. *)
+(*   destruct cmd; ss; *)
+(*     inv STEP; ss; *)
+(*       des; esplits; eauto. *)
+(*   admit. (* easy *) *)
+(* Admitted. *)
+
+
+
+(* Lemma inject_event_implies_mem_change_inject *)
+(*       m_src conf_src st0_src mc_src cmd_src *)
+(*       m_tgt conf_tgt st0_tgt mc_tgt cmd_tgt *)
+(*       invst0 invmem0 inv0 *)
+(*       (CONF: InvState.valid_conf m_src m_tgt conf_src conf_tgt) *)
+(*       (STATE : InvState.Rel.sem conf_src conf_tgt st0_src st0_tgt invst0 invmem0 inv0) *)
+(*       (MEM : InvMem.Rel.sem conf_src conf_tgt (Mem st0_src) (Mem st0_tgt) invmem0) *)
+(*       (INJECT: postcond_cmd_inject_event cmd_src cmd_tgt inv0 = true) *)
+(*       (MEM_CH_REL_SRC: mem_change_cmd conf_src st0_src mc_src cmd_src) *)
+(*       (MEM_CH_REL_TGT: mem_change_cmd conf_tgt st0_tgt mc_tgt cmd_tgt) *)
+(*   : mem_change_inject conf_src conf_tgt invmem0 mc_src mc_tgt. *)
+(* Proof. *)
+(*   destruct cmd_src; destruct cmd_tgt; ss; *)
+(*     (try by des; subst; econs); des; subst; simtac; *)
+(*       (try by exploit_inject_value; inv_conf; inject_clarify; econs; eauto). *)
+(*   unfold Invariant.is_private in *. des_ifs. *)
+(*   destruct x as [t x]; unfold ValueT.lift in *. des_ifs. *)
+(*   inv STATE. inv SRC. *)
+(*   exploit PRIVATE. *)
+(*   { apply IdTSet.mem_2; eauto. } *)
+(*   { inv_conf. *)
+(*     inject_clarify. *)
+(*   } *)
+(*   i. des_ifs. *)
+(*   econs; eauto. *)
+(* Qed. *)
+
+
+(* Lemma step_mem_change_inject *)
+(*       m_src conf_src st0_src st1_src evt_src cmd_src cmds_src  *)
+(*       m_tgt conf_tgt st0_tgt st1_tgt evt_tgt cmd_tgt cmds_tgt  *)
+(*       invst0 invmem0 inv0 inv1 *)
+(*       (CONF: InvState.valid_conf m_src m_tgt conf_src conf_tgt) *)
+(*       (STATE: InvState.Rel.sem conf_src conf_tgt st0_src st0_tgt invst0 invmem0 inv0) *)
+(*       (MEM: InvMem.Rel.sem conf_src conf_tgt st0_src.(Mem) st0_tgt.(Mem)invmem0) *)
+(*       (NONCALL_SRC: Instruction.isCallInst cmd_src = false) *)
+(*       (NONCALL_TGT: Instruction.isCallInst cmd_tgt = false) *)
+(*       (CMDS_SRC: CurCmds st0_src.(EC) = cmd_src :: cmds_src) *)
+(*       (CMDS_TGT: CurCmds st0_tgt.(EC) = cmd_tgt :: cmds_tgt) *)
+(*       (FORGET_SRC: inv_unary_forgot inv1.(Invariant.src) (AtomSetImpl_from_list (option_to_list (Cmd.get_def cmd_src)))) *)
+(*       (FORGET_TGT: inv_unary_forgot inv1.(Invariant.tgt) (AtomSetImpl_from_list (option_to_list (Cmd.get_def cmd_tgt)))) *)
+(*       (STEP_SRC: sInsn conf_src st0_src st1_src evt_src) *)
+(*       (STEP_TGT: sInsn conf_tgt st0_tgt st1_tgt evt_tgt) *)
+(*       (INJECT: postcond_cmd_inject_event cmd_src cmd_tgt inv0 = true) *)
+(*   : exists mc_src mc_tgt, *)
+(*     <<MEM_CH_INJECT: mem_change_inject conf_src conf_tgt invmem0 mc_src mc_tgt>> /\ *)
+(*     <<MEM_CH_CMD_SRC: mem_change_cmd_after conf_src (mkState st1_src.(EC) st1_src.(ECS) st0_src.(Mem)) mc_src cmd_src inv1.(Invariant.src)>> /\ *)
+(*     <<MEM_CH_CMD_TGT: mem_change_cmd_after conf_tgt (mkState st1_tgt.(EC) st1_tgt.(ECS) st0_tgt.(Mem)) mc_tgt cmd_tgt inv1.(Invariant.tgt)>> /\ *)
+(*     <<STATE_EQUIV_SRC: state_equiv_except_mem conf_src (mkState st1_src.(EC) st1_src.(ECS) st0_src.(Mem)) st1_src mc_src>> /\ *)
+(*     <<STATE_EQUIV_TGT: state_equiv_except_mem conf_tgt (mkState st1_tgt.(EC) st1_tgt.(ECS) st0_tgt.(Mem)) st1_tgt mc_tgt>>. *)
+(* Proof. *)
+(*   destruct cmd_src; inv STEP_SRC; ss. *)
+(*   Time destruct cmd_src eqn:CMD_SRC; destruct cmd_tgt eqn:CMD_TGT; ss; *)
+(*     destruct st0_src; destruct EC0; inv STEP_SRC. *)
+(*     inv STEP_SRC. *)
+  
+(*   destruct st0_src; ss. destruct EC0; ss. inv STEP_SRC; ss. *)
+(*     try inv STEP_SRC; ss; inv STEP_TGT; ss. *)
+(*       esplits; auto; *)
+(*         econs; ss; econs; ss. *)
+(*       - inv STEP_SRC; ss; inv STEP_TGT; ss; *)
+(*       esplits; auto; *)
+(*         econs; ss; econs; ss. *)
+(*       - inv STEP_SRC; ss; inv STEP_TGT; ss; *)
+(*       esplits; auto; *)
+(*         econs; ss; econs; ss. *)
+  
+(*     try by inv STEP_SRC; ss; inv STEP_TGT; ss; *)
+(*       esplits; auto; *)
+(*         econs; ss; econs; ss. *)
+(*     esplits; eauto. *)
+(*     + econs. *)
+(*     + econs; ss. *)
+(*       inv STEP_SRC; ss. *)
+(*       econs; ss. *)
+(*     + econs; ss. *)
+(*       inv STEP_TGT; ss. *)
+(*       econs; ss. *)
+
+(*     admit. (* nop nop *) *)
+(*   - *)
+(*   unfold postcond_cmd_inject_event in *. *)
+  
+(* Admitted. *)
+
+
+(* Lemma step_equiv_except_mem *)
+(*       conf st0 st1 evt *)
+(*       cmd cmds *)
+(*       invst0 invmem0 inv0 inv1 *)
+(*       public gmax *)
+(*       (STATE: InvState.Unary.sem conf st0 invst0 invmem0 inv0) *)
+(*       (STATE_FORGET: InvState.Unary.sem conf (mkState st1.(EC) st1.(ECS) st0.(Mem)) invst0 invmem0 inv1) *)
+(*       (MEM: InvMem.Unary.sem conf gmax public st0.(Mem) invmem0) *)
+(*       (NONCALL: Instruction.isCallInst cmd = false) *)
+(*       (CMDS: CurCmds st0.(EC) = cmd :: cmds) *)
+(*       (FORGET: inv_unary_forgot inv1 (AtomSetImpl_from_list (option_to_list (Cmd.get_def cmd)))) *)
+(*       (STEP: sInsn conf st0 st1 evt) *)
+(*   : exists mc, *)
+(*     <<MEM_CH_CMD: mem_change_cmd_after conf (mkState st1.(EC) st1.(ECS) st0.(Mem)) mc cmd inv1>> /\ *)
+(*                   <<STATE_EQUIV: state_equiv_except_mem conf (mkState st1.(EC) st1.(ECS) st0.(Mem)) st1 mc>>. *)
+(* Proof. *)
+(*   inv STEP; destruct cmd; inv CMDS; ss; *)
+(*     try by esplits; eauto; econs; eauto; econs; eauto. *)
+(*   - admit. (* malloc *) *)
+(*   - esplits; eauto. *)
+(*     econs; eauto. *)
+(*     econs; eauto. *)
+(*     + admit. (* malloc , should know newly allocated block is unique *) *)
+(*     + ss. apply lookupAL_updateAddAL_eq. *)
+(* Admitted. *)
